powerpc/SelectLongproof.v
@@ -1,0 +1,22 @@
+(* *********************************************************************)
+(*                                                                     *)
+(*              The Compcert verified compiler                         *)
+(*                                                                     *)
+(*                 Xavier Leroy, INRIA Paris                           *)
+(*                                                                     *)
+(*  Copyright Institut National de Recherche en Informatique et en     *)
+(*  Automatique.  All rights reserved.  This file is distributed       *)
+(*  under the terms of the INRIA Non-Commercial License Agreement.     *)
+(*                                                                     *)
+(* *********************************************************************)
+
+(** Instruction selection for 64-bit integer operations *)
+
+Require Import String Coqlib Maps Integers Floats Errors.
+Require Archi.
+Require Import AST Values Memory Globalenvs Events.
+Require Import Cminor Op CminorSel.
+Require Import SelectOp SelectOpproof SplitLong SplitLongproof.
+Require Import SelectLong.
+
+(** This file is empty because we use the default implementation provided in [SplitLong]. *)
